## Functions
Functions can be thought of as a collection of ordered pairs. They map an element in their **domain** to another element in their **range**.

>[!INFO] Definition 2.3.1
>**Function:** Let $A,B$ be nonempty sets. A **function** $f$ from $A$ to $B$ is the rule that assigns exactly one element of B to each element of A.
>
>Denoted $f:\ A \rightarrow B$. If $a \in A$ and $b \in B$, we have $f(a) = b$.

Functions generally take the form of: $f=\{(a,b):\ a \in A, b \in B\}$.
	Ex: $f(x^{2}) \rightarrow f=\{(x,x^{2}):\ x \in \mathbb{R}, x^{2} \in \mathbb{R_{\geq 0}}\}$

>[!TIP] From algebra, recall that a function can only have one output for each input.

>[!EXAMPLE] Example 2.3.1
>**Determine if each $f$ is a function from $\mathbb{Z}$ to $\mathbb{R}$.**
>
>1. $f(x)=\frac{1}{x}$
>	- We can't set $x=0$, so *not a function*.
>2. $f(n)=\pm n$
>	- Multiple outputs for each input, so *not a function*.
>3. $f(n) = \sqrt{n^{2}+1}$
>	- *Yes*, this is a function.

## Domain, Codomain, Range
>[!INFO] Definitions 2.3.2
>**Domain:** Set in which the inputs of a function lie.
>**Codomain:** Set in which the optus of a function lie.
>
>Let $f:\ A \rightarrow B$ be a function. $A$ is the **Domain**, and $B$ is the **Codomain**.

If $f(a)=b$, then $b$ is the **image** of $a$ under $f$, and $a$ is the **preimage** of $b$ under $f$.

>[!INFO] Definition 2.3.3
>**Range:** The **range** of a function is the subset of its codomain that consists of images of elements of its domain.
>
>If we have a function $f:\ A \rightarrow B$, the **Range** of $f$ is the subset of $B$ consiting of **images** of elements of $A$.

The range and codomain are sometimes the same, but not always!
	Ex: Let $A=\{car,\ train,\ plane\}$ and $B=\{apple,\ orange\}$, and let $f$ be the rule that sends $car$ to $apple$, train to apple, and plane to apple. In this function from A to B, the **domain** is $\{car,\ train,\ plane\}$, the **codomain** is $\{apple,\ orange\}$, and the **range** is $\{apple\}$.
	Ex: Let $f:\ \mathbb{N} \rightarrow \mathbb{N}$ be defined by $f(n) = 2n$. The **domain** is $\mathbb{N}$, the **codomain** is $\mathbb{N}$, and the **range** is the nonnegative even integers. In this case, $2$ is the **image** of $1$, and $1$ is the **preimage** of $2$.

>[!EXAMPLE] Example 2.3.2
>**Determine the domain and codomain/range of the following.**
>
>1. $f$ assigns to each integer its last digit. 
>	- Domain: $\mathbb{Z}$
>	- Range: $\{0,1,\dots , 9\}$
>2. $f$ assigns to each positive integer the largest perfect square not exceeding the integer.
>	- Domain: $\mathbb{Z_{>0}}$
>	- Range: $\{1,4,9,\dots\} = \{m^{2} \in \mathbb{Z_{\geq 1}}\}$
>3. $f$ assigns to each pair of integers the first integer in the pair.
>	- Domain: $\mathbb{Z} \times \mathbb{Z} = \mathbb{Z}^{2}$
>	- Range: $\mathbb{Z}$

## Injective, Surjective, Bijective
>[!INFO] Definition 2.3.4
>**Injective:** $f$ is **injective** or **one-to-one** if whenever $f(a_{1})=f(a_{2})$, then $a_{1} = a_{2}$.

To show a function is not injective, find 2 elements $a_{1}, a_{2} \in A$ with $a_{1} \neq a_{2}$ but $f(a_{1}) = f(a_{2})$.
	Ex: If $f:\ \mathbb{Z} \rightarrow \mathbb{N}$ is a function defined by $f(n)=n^{2}$, $f$ is not injective, as $f(1)=1=f(-1)$, however $-1 \neq 1$.

>[!EXAMPLE] Example 2.3.3
>**Let $f:\ \mathbb{N} \rightarrow \mathbb{N}$ be a function defined by $f(n)=2n$. Prove injective.**
>
>*Proof:* Let $f(m)=f(n)$ for some $m,n \in \mathbb{N}$. This means that $2m = 2n$, i.e., $2m-2n = 0$. Since $2 \neq 0$, we have $m-n=0$, i.e., $m=n$. Thus, $f$ is injective. $\square$

>[!TIP] Injective proofs always start "Let $f(a_{1})=f(a_{2})$ for some $a_{1},a_{2}\in A$" and show $a_{1}=a_{2}$.

>[!INFO] Definition 2.3.5
>**Surjective:** $f$ is **surjective** or **onto** if the codomain is equal to the range, i.e., for every $b \in B$, there exists $a \in A$ so that $f(a) = b$.

To show a function is not surjective, find element $b \in B$ so that there is not $a \in a$ with $f(a)=b$.
	Ex: If $f:\ \mathbb{N} \rightarrow \mathbb{N}$ is a function defined by $f(n)=2n$, then $f$ is not surjective, as $1 \in \mathbb{N}$, but there is no $n$ such that $f(n)=1$. (In this case, $2n=1$ has no solutions)

>[!EXAMPLE] Example 2.3.4
>**Let $f:\ \mathbb{R} \rightarrow \mathbb{R_{\geq 0}}$ be defined by $f(x)=x^2$ where $\mathbb{R_{\geq 0}}=\{x \in \mathbb{R}:\ x \geq 0\}$. Prove Surjective.**
>
>*Proof:* Let $x \in \mathbb{R_{\geq 0}}$. We have $\sqrt{x} \in \mathbb{R}$ and $f(\sqrt{x})$, so $f$ is surjective. $\square$

>[!TIP] Surjective proofs always start "Let $b \in B$" and find $a \in A$ so that $f(a)=b$.

>[!INFO] Definition 2.3.6
>**Bijective:** $f$ is **bijective** is it is both injective and surjective.

![[injective-surjective-bijective.png]]
Following nicely from the definition, proving a function is bijective requires proving that it is both injective and surjective.

>[!EXAMPLE] Example 2.3.5
>**Let $f: \mathbb{Z} \rightarrow \mathbb{Z}$ be defined by $f(n) = n+1$. Prove bijective.**
>
>*Injective:* Let $f(m)=f(n)$ for some $m,n \in \mathbb{Z}$. This means that $m+1=n+1$. Subtracting $1$ from each side gives us $m=n$. Thus, $f$ is injective.
>
>*Surjective:* Let $m \in \mathbb{Z}$. We have $m-1 \in \mathbb{Z}$ and $f(m-1)=(m-1)+1=m$. Thus, $f$ is surjective.
>
>Since we have proven that $f$ is both injective and surjective, $f$ is bijective. $\square$

## Composition and Inverse
>[!INFO] Definition 2.3.7
>**Composition:** Let $f:\ A \rightarrow B$ and $g:\ B \rightarrow C$. The **composition** of $f$ and $g$ is given by $g \circ f:\ A \rightarrow C$.
>
>In this notation, we find $(g \circ f)(a)=g(f(a))$

In the composition of functions $f$ and $g$, the codomain of $f$ (inner function) must be the domain of $g$ (inner function).

>[!INFO] Definition 2.3.8
>**Inverse:** Let $f:\ A \rightarrow B$ be a bijective function. The **Inverse Function** of $f$ $f^{-1}:\ B \rightarrow A$. In other words, the domain and codomain are swapped.

For a bijective function, if $f(a)=b$, then $f^{-1}(b)=a$.

Composing a function with its inverse gives an identity. I.e., $(f \circ f^{-1})(a)=a$ for every $a \in A$.

>[!EXAMPLE] Example 2.3.6
>**We have a bijective function $f:\ \mathbb{Z} \rightarrow \mathbb{Z}$ given by $f(n)=n+1$. Show that $f:\ \mathbb{Z} \rightarrow \mathbb{Z}$ given by $f^{-1}(n)=n-1$ is its inverse.**
>
>We have: $$\begin{align*}
>	(f^{-1} \circ f)(n)&= f^{-1}(f(n))\\
>	&= f^{-1}(n+1)\\
>	&= (n+1)-1 = n.
>	\end{align*}$$
>Similarly, we have: $$\begin{align*}
>	(f \circ f^{-1})(n)&= f(f^{-1}(n))\\
>	&= f(n-1)\\
>	&= (n-1)+1 = n.
>	\end{align*}$$ Thus, we find that $f^{-1}$ is the inverse of $f$.

## More Examples
 >[!EXAMPLE] Example 2.3.7
 >**Determine if the following is injective. If so, prove it.**
 >
 >1. $A=\{a,b,c,d\}$, Define $f:\ A \rightarrow A$ with $f(a)=b, f(b)=a, f(c)=c, f(d)=d$.
>	- *Proof:* By inspection, we see each output of $f$ is distinct. Thus, $f$ is injective. $\square$
>2. Let $f:\ \mathbb{Z} \rightarrow \mathbb{Z}$ be defined by $f(n)=n+2$.
>	- *Proof:* Let $m,n\in \mathbb{Z}$. This means that $m+2=n+2$, i.e., $m=n$. Thus, $f$ is injective. $\square$
>3. Let $f:\ \mathbb{Z} \rightarrow \mathbb{Z}$ be defined by $f(n)=\lceil \frac{n}{2} \rceil$.
>	- NOT Injective, because $f(1)=\lceil \frac{1}{2} \rceil = 1$ and $f(2)=\lceil \frac{2}{2} \rceil = 1$.
>4. $A=\{a,b,c,d\}$, Define $f:\ A \rightarrow A$ with $f(a)=b, f(b)=b, f(c)=d, f(d)=c$.
>	- NOT Injective, because $f(a)=b$ and $f(b)=b$.
>5. Let $f:\ \mathbb{Z} \rightarrow \mathbb{Z}$ be defined by $f(n)=n^3$.
>	- *Proof:* Let $m,n \in \mathbb{Z}$ and assume $f(m)=f(n)$. This means that $m^3=n^3$, i.e., $m^3-n^3=0$. Thus, $(m-n)(m^2+mn+n^2)=0$. Either $m-n=0$, i.e., $m=n$ and we are done, or $m^2+mn+n^2=0$. But $m^2+mn+n^2=0$ only if $m=n=0$. In either case, $m=n$, Thus, $f$ is injective. $\square$

>[!EXAMPLE] Example 2.3.8
>**Determine if the following is surjective. If so, prove it.**
>
>1. $f: \mathbb{Z} \times \mathbb{Z} \rightarrow \mathbb{Z}$ defined by $f(m,n)=2m-n$.
>	- *Proof:* Let $n \in \mathbb{Z}$. We have $f(n,n)=2n-n=n$. Thus, $f$ is surjective. $\square$
>2. $f: \mathbb{Z} \times \mathbb{Z} \rightarrow \mathbb{Z_{\geq 0}}$ defined by $f(m,n)=m^2+n^2$.
>	- NOT Surjective. Note $m^{2}+n^{2} \neq 3$ by inspection.
>3. $f: \mathbb{Z} \times \mathbb{Z} \rightarrow \mathbb{Z}$ defined by $f(m,n)=m+n-1$.
>	- *Proof:* Let $a \in \mathbb{Z}$. We have $f(a,1)=a+1-1=a$. Thus, $f$ is surjective. $\square$
>4. $f: \mathbb{Z} \times \mathbb{Z} \rightarrow \mathbb{Z_{\geq -4}}$ defined by $f(m,n)=m^2-4$.
>	-NOT Surjective. $f(m,n)=-1$ implies $m^{2}-4=-1 \Rightarrow m^2=3$.

>[!EXAMPLE] Example 2.3.9
>**Let $f:\ A \rightarrow B$ and $g:\ B \rightarrow C$ be surjective. Prove $g \circ f:\ A \rightarrow C$ is surjective.**
>
>*Proof:* Let $c \in C$. Since $g$ is surjective, there exists $b \in B$ such that $g(b)=c$. Since $f$ is surjective, there exists $a \in A$ so that $f(a)=b$. Observe that we have $g(f(a))=g(b)=c$. Thus, $g \circ f$ is surjective. $\square$

>[!EXAMPLE] Example 2.3.10
>**Let $f:\ A \rightarrow B$ and $g:\ B \rightarrow C$ be injective. Prove $g \circ f:\ A \rightarrow C$ is injective.**
>
>*Proof:* Assume $(g \circ f)(m)=(g \circ f)(n)$, i.e., $g(f(m))=g(f(n))$ for some $m,n \in A$. Because $g$ is injective, we have $f(m) = f(n)$. Because $f$ is injective, we have $m=n$. Thus, $g \circ f$ is injective. $\square$

>[!EXAMPLE] Example 2.3.11
>**Let $f:\ A \rightarrow B$ be a function and $S,T \subseteq A$. Prove $f(S \cup T) = f(S) \cup f(T)$.**
>
>*Proof:* Let $x \in f(S \cup T)$. So $x = f(a)$ for some $a \in (S \cup T)$. If $a \in S$, then $f(a)=f(S)$, so $x \in f(S)$. If $a \in T$, then $f(a)=f(T)$, so $x \in f(T)$. Thus, $x \in f(S) \cup f(T)$, and therefore $f(S \cup T) \subseteq f(S) \cup f(T)$. Now, let $x \in f(S) \cup f(T)$. This means that $x \in f(S)$ or $x \in f(T)$. If $x \in f(S)$, then $x=f(s)$ for some $s \in S$. But $S \subseteq S \cup T$, so $s \in S \cup T$. Thus, $x \in f(S \cup T)$. If $x \in f(T)$, then $x = f(t)$ for some $t \in T$. But $T \subseteq S \cup T$, so $t \in S \cup T$. Thus, $x \in f(S \cup T)$, and therefore $f(S) \cup f(T) \subseteq f(S \cup T)$. Hence, $f(S \cup T) = f(S) \cup f(T)$. $\square$

This next problem was originally on homework #4, but worked through in class, as most people had incorrect proofs.
>[!EXAMPLE] Example 2.3.12
>**Let $g:\ A \rightarrow B$ and $f:\ B \rightarrow C$.  Prove that if $f \circ g$ is a bijection, then $g$ is onto if and only if $f$ is injective.**
>
>*Proof:*
>"$\Rightarrow$" Assume $g$ is surjective. Let $b_{1},b_{2} \in B$ and assume $f(b_{1})=f(b_{2})$. Since $g$ is surjective, there exists $a_{1},a_{2} \in A$ so that $g(a_{1})=b_{1}$ and $g(a_{2})=b_{2}$. We have $(f \circ g)(a_{1})=f(g(a_{1}))=f(b_{1})$ and $(f \circ g)(a_{2})=f(g(a_{2}))=f(b_{2})$. Since $f(b_{1})=f(b_{2})$ by assumption, $f(g(a_{1}))=f(g(a_{2}))$. As $f \circ g$ is bijective, it is injective, so $a_{1}=a_{2}$. Thus, $g(a_{1})=g(a_{2})$, i.e., $b_{1}=b_{2}$. Therefore, $f$ is injective.
>"$\Leftarrow$" Assume $f$ is injective. Let $b \in B$. Let $c=f(b) \in C$. As $f \circ g$ is bijective, it is surjective, so there exists $a \in A$ so that $(f \circ g)(a)=c$. So, $g(a)=b'$ for some $b' \in B$. Observe $f(b')=f(g(a))=c$. Thus, $f(b)=c=f(b')$, and $f$ injective means that $b=b'$. Hence, $g(a)=b=b'$, so $g$ is surjective. $\square$
