For simplicity, let's pretend the alphabet is only 6 letters long: $\mathbb{Z}/6\mathbb{Z}=\{A,B,C,D,E,F\}=\{[0]_{6},[1]_{6},[2]_{6},[3]_{6},[4]_{6},[5]_{6}\}$.

If we want to do a Caesar shift of $+2$, it would look like this:

| A               |                    | B            |                    | C            |                    | D            |                    | E            |                    | F            |
| --------------- | ------------------ | ------------ | ------------------ | ------------ | ------------------ | ------------ | ------------------ | ------------ | ------------------ | ------------ |
| $+2 \downarrow$ |                    | $\downarrow$ |                    | $\downarrow$ |                    | $\downarrow$ |                    | $\downarrow$ |                    | $\downarrow$ |
| C               | $\xrightarrow{+1}$ | D            | $\xrightarrow{+1}$ | E            | $\xrightarrow{+1}$ | F            | $\xrightarrow{+1}$ | A            | $\xrightarrow{+1}$ | B            | 

We can think of the Caesar Cipher as adding the key to the first letters, and all other letters add one to their value based on that. In other words, we add 2 vertically and 1 horizontally.

## Encryption

For an **Affine Cipher**, we don't just add 1 in the bottom row. What if we try adding 2 vertically and 3 horizontally?

| A               |                    | B            |                    | C            |                    | D            |                    | E            |                    | F            |
| --------------- | ------------------ | ------------ | ------------------ | ------------ | ------------------ | ------------ | ------------------ | ------------ | ------------------ | ------------ |
| $+2 \downarrow$ |                    | $\downarrow$ |                    | $\downarrow$ |                    | $\downarrow$ |                    | $\downarrow$ |                    | $\downarrow$ |
| C               | $\xrightarrow{+3}$ | F            | $\xrightarrow{+3}$ | C            | $\xrightarrow{+3}$ | F            | $\xrightarrow{+3}$ | C            | $\xrightarrow{+3}$ | F            |

This doesn't actually work: the cipher text will only have C and F, so it will be impossible to go back to the plaintext. Also, notice $gcd(3,6)=2$, which doesn't work. For now, we can observe that the encryption function $e$ must be injective, and it appears that the $gcd$ of the horizontal key and the size of the alphabet must be $1$ as well. Let's try another, with 2 vertically and 5 horizontally:

| A               |                    | B            |                    | C            |                    | D            |                    | E            |                    | F            |
| --------------- | ------------------ | ------------ | ------------------ | ------------ | ------------------ | ------------ | ------------------ | ------------ | ------------------ | ------------ |
| $+2 \downarrow$ |                    | $\downarrow$ |                    | $\downarrow$ |                    | $\downarrow$ |                    | $\downarrow$ |                    | $\downarrow$ |
| C               | $\xrightarrow{+5}$ | B            | $\xrightarrow{+5}$ | A            | $\xrightarrow{+5}$ | F            | $\xrightarrow{+5}$ | E            | $\xrightarrow{+5}$ | D            | 

Here, the encryption is 1:1, and $gcd(5,6)=1$, so this **Affine Cipher** works. Since we know now that our encryption function must be injective and our decryption function must be the inverse of our encryption function, so our encryption function $e$ must be *bijective*.

>[!ABSTRACT] Fact
>**If $f:\ A \rightarrow B$ and $\#A = \#B < \infty$, then $f$ is injective iff $f$ is surjective iff $f$ is bijective.**

Before we formally define the **Affine Cipher**, we need to determine how to represent it mathematically. Let's look at the previous table again, but this time with equivalence classes:

| A$=[0]_{6}$  |                    | B$=[1]_{6}$            |                    | C$=[2]_{6}$            |                    | D$=[3]_{6}$            |                    | E$=[4]_{6}$            |                    | F$=[5]_{6}$            |
| --------------- | ------------------ | ------------ | ------------------ | ------------ | ------------------ | ------------ | ------------------ | ------------ | ------------------ | ------------ |
| $+2 \downarrow$ |                    | $\downarrow$ |                    | $\downarrow$ |                    | $\downarrow$ |                    | $\downarrow$ |                    | $\downarrow$ |
| C$=[2]_{6}$               | $\xrightarrow{+5}$ | B$=[1]_{6}$            | $\xrightarrow{+5}$ | A$=[0]_{6}$            | $\xrightarrow{+5}$ | F$=[5]_{6}$            | $\xrightarrow{+5}$ | E$=[4]_{6}$            | $\xrightarrow{+5}$ | D$=[3]_{6}$            |

Here, we have $e([n]_{6})=[5n+2]_{6}$. We can generalize this function into a formal definition for the whole alphabet.

>[!INFO] Definition 4.3.1
>**Affine Cipher:** A substitution cipher with encryption function $e([n]_{26})=[an+b]_{26}$ with $a,b\in \mathbb{Z}$ and $gcd(a,b)=1$.
>
>We would say that this is an "affine cipher of a, b".

>[!EXAMPLE] Example 4.3.1
>**Encrypt "ENCRYPTION" with $e([n]_{26})=[7n+3]_{26}$.**
>
>E $=[7(4)+3]_{26}=[31]_{26}=[5]_{26}=$ F
>N $=[7(13)+3]_{26}=[16]_{26}=$ Q
>C $=[7(2)+3]_{26}=[17]_{26}=$ R
>R $=[7(17)+3]_{26}=[18]_{26}=$ S
>Y $=[7(24)+3]_{26}=[15]_{26}=$ P
>P $=[7(15)+3]_{26}=[4]_{26}=$ E
>T $=[7(19)+3]_{26}=[6]_{26}=$ G
>I $=[7(8)+3]_{26}=[7]_{26}=$ H
>O $=[7(14)+3]_{26}=[23]_{26}=$ X
>N $=[7(13)+3]_{26}=[16]_{26}=$ Q
>
>"ENCRYPTION" = FQRSPEGHXQ.

## Decryption
How do we decrypt an Affine Cipher? Let's look at the cipher from the previous example: $$\begin{align*}
	[m]_{26} &= [7n+3]_{26}\\
	7n+3 &\equiv m \pmod{26}\\
	7n &\equiv m-3 \pmod{26}.
\end{align*}$$Because we are working in $\mathbb{Z}/26\mathbb{Z}$, we can't divide both sides by $7$ to find the result. Instead, we need to find the **multiplicative inverse** of 7, which can be represented as $7^{-1}$.

### Multiplicative Inverse
>[!INFO] Definition 4.3.2
>**Multiplicative Inverse:** For $n \in A$, the **multiplicative inverse** is the value $n^{-1}$ such that $n\cdot n^{-1}=1$.

In $\mathbb{R}, \mathbb{Z}$, and many other infinite planes, $n^{-1}=\frac{1}{n}$. In $\mathbb{Z}/n\mathbb{Z}$, however, we must find a **multiplicative inverse** such that $[a]_{n}^{-1} \cdot [a]_{n}=1$. In other words, what must we multiply $[a]_{n}$ by to get the answer $1$? We can find this by applying the euclidean algorithm with back substitution to $gcd(a,26)$, as we know that the $gcd$ of an affine cipher is always $1$. Let's continue with our previous example, using $gcd(7,26)$: $$\begin{align*}
	26 &= 7(3)+5\\
	7 &= 5(1)+2\\
	5 &= 2(2)+1.
\end{align*}$$Notice that we can stop here, as our final $r=1$ tells us that our $gcd$ is $1$, which we already know to be true. Now, we use back substitution: $$\begin{align*}
	1 &= 5+2(-2)\\
	1 &= 5+(7+5(-1))(-2)\\
	1 &= 5(3)+7(-2)\\
	1 &= (26+7(-3))(3)+7(-2)\\
	1 &= 26(3)+7(-11).
\end{align*}$$Finally, let's convert this linear combination to equivalence classes in $\mathbb{Z}/26\mathbb{Z}$. The first term will disappear (as $[26]_{26}=[0]_{26}$), which will leave us with our desired **multiplicative inverse**: $$\begin{align*}
	[1]_{26} &= [26(3)+7(-11)]_{26}\\
	[1]_{26} &= [26]_{26}[3]_{26}+[7]_{26}[-11]_{26}\\
	[1]_{26} &= [7]_{26}[-11]_{26}\\
	[1]_{26} &= [7]_{26}[15]_{26}.
\end{align*}$$ Thus, we find that the **multiplicative inverse** of $7$ is $15$ in $\mathbb{Z}/26\mathbb{Z}$.

We can use this information to finally find our decryption function: $$\begin{align*}
	[m]_{26} &= [7n+3]_{26}\\
	7n+3 &\equiv m \pmod{26}\\
	7n &\equiv m-3 \pmod{26}\\
	7(15)n &\equiv 15(m-3) \pmod{26}\\
	n &\equiv 15(m-3) \pmod{26}.
\end{align*}$$Finally, we find our decryption function $d([m]_{26})=[15(m-3)]_{26}$. We can generalize this function into a broader definition for the decryption function.

>[!INFO] Definition 4.3.3
>**Affine Decryption Function:** For an Affine Cipher $e([n]_{26})=[an+b]_{26}=[m]_{26}$, we find the **decryption function** to be $d([m]_{26})=[a^{-1}(m-b)]_{26}=[n]_{26}$.

>[!EXAMPLE] Example 4.3.2
>**$e([n]_{26})=[11n+6]_{26}$. Decrypt "JLQNGK".**
>
>Find the decryption function: $$\begin{align*}
>	11n+6 &\equiv m \pmod{26}\\
>	11n &\equiv m-6 \pmod{26}\\\\
>	
>	gcd(11,26) &= 1\\
>	26 &= 11(2)+4\\
>	11 &= 4(2)+3\\
>	4 &= 3(1)+1\\\\
>	
>	1 &= 4+3(-1)\\
>	1 &= 4+(11+4(-2))(-1)\\
>	1 &= 4(3)+11(-1)\\
>	1 &= (26+11(-2))(3)+11(-1)\\
>	1 &= 26(3)+11(-7)\\
>	[1]_{26} &= [26]_{26}[3]_{26}+[11]_{26}[-7]_{26}\\
>	[1]_{26} &= [11]_{26}[-7]_{26}\\
>	[1]_{26} &= [11]_{26}[19]_{26}\\\\
>	
>	11n &\equiv m-6 \pmod{26}\\
>	11(19)n &\equiv 19(m-6) \pmod{26}\\
>	n &\equiv 19(m-6) \pmod{26}
>	\end{align*}$$Our decryption function is $d([m]_{26})=[19(m-6)]_{26}$
>	
>Decrypt each letter:
>J $=[19(9-6)]_{26}=[17]_{26}=$ F
>L $=[19(11-6)]_{26}=[17]_{26}=$ R
>Q $=[19(16-6)]_{26}=[17]_{26}=$ I
>N $=[19(13-6)]_{26}=[17]_{26}=$ D
>G $=[19(6-6)]_{26}=[17]_{26}=$ A
>K $=[19(10-6)]_{26}=[17]_{26}=$ Y
>
>"JLQNGK" = FRIDAY.





